SP1Chips/LtChip.lean
@@ -42,17 +42,13 @@ theorem correct_slt
   let op_a := sp1_op_a Main
   (spec_slt (.Regidx op_c) (.Regidx op_b) (.Regidx op_a)).run s = (sp1_slt Main).run s
   := by
-    have _ := state_cstrs
-    have _ := cstrs
-    have _ := h_is_slt
-    stop
     simp [SP1ConstraintList.allHold] at cstrs; simp [is_slt] at h_is_slt
     rw [allHold_constraints_iff_slt h_is_slt] at cstrs
-    obtain ⟨lt_op_cstrs, cpu_cstrs, alu_cstrs, M33⟩ := cstrs
+    obtain ⟨lt_op_cstrs, cpu_cstrs, alu_cstrs, M33, _M13⟩ := cstrs
     have h_is_real : Main[32] + Main[33] = 1 := by simp_all
     rw [CPUState.allHold_constraints_iff_is_real h_is_real] at cpu_cstrs
     rw [ALUTypeReader.allHold_constraints_iff_is_real h_is_real] at alu_cstrs
-    obtain ⟨ _, trusted_instr_prop, _, _, _, _, _, _, _, _, _, _, _, _, _, _, is_U64_a, is_U64_b, is_U64_c , _, _ ⟩ := alu_cstrs
+    obtain ⟨ trusted_instr_prop, _, _, _, _, _, _, _, _, _, _, _, _, _, _, is_U64_a, is_U64_b, is_U64_c , _, _ ⟩ := alu_cstrs
     simp [SP1ConstraintList.initialState, constraints, SP1Constraint.toStateProp, List.Forall, CPUState.constraints, ALUTypeReader.constraints] at state_cstrs
     obtain ⟨throwaway, read_pc, read_op_a, read_op_b, read_op_c⟩ := state_cstrs
     clear throwaway; simp_all
@@ -63,10 +59,10 @@ theorem correct_slt
     rw [Sail.run_readReg, read_pc]
     simp [sp1_op_a, sp1_op_b, sp1_op_c, read_op_b, read_op_c]
     rw [exec_RTYPE_pure_bv_to_w _ _ _ (by omega) (by omega)]
-    by_cases h_is_op_a_0 : Main[6] = 0 <;> simp_all
-    · simp [Word.toBitVec64, Word.toNat]
-      exact Fin.BitVec_ofNat_add_eq_add_ofNat _ 4 (by decide) (by omega)
-    · rw [if_neg (by simp [← BitVec.toNat_inj]; omega)]
+    by_cases h_is_op_a_0 : Main[6] = 0
+    · simp_all
+    · simp_all
+      rw [if_neg (by simp [← BitVec.toNat_inj]; omega)]
       rw [if_neg (c := BitVec.ofNat 5 ↑Main[6] = 0#5) (by simp [← BitVec.toNat_inj]; omega)]
       apply LtOperationSigned.spec.signed at lt_op_cstrs <;>
       [ simp_all; exact is_U64_b; exact is_U64_c ]
@@ -83,63 +79,20 @@ open Lt
 variable
   (Main : Vector (Fin KB) 44)
   (s : SailState)
-  (cstrs : (constraints Main).allHold)
-  (h_is_sltu : is_sltu Main)
 
 def spec_slti (imm : BitVec 12) (rs1 rd : regidx) : SailM Unit := do
   Sail.writeReg Register.nextPC ((← Sail.readReg Register.PC) + 4#64)
   _ ← execute_ITYPE imm rs1 rd iop.SLTI
   pure ()
 
-def sp1_op_a : BitVec 5 :=
-  by
-    have _ := Main
-    have _ := cstrs
-    have _ := h_is_sltu
-    stop
-    refine BitVec.ofNatLT Main[6] ?_
-    change Main[6] < 32
-    rw [SP1ConstraintList.allHold, allHold_constraints_iff_sltu h_is_sltu] at cstrs
-    obtain ⟨ lt_op, cpu, alu, rest ⟩ := cstrs
-    simp [ALUTypeReader.constraints, SP1Constraint.toProp] at alu
-    simp_all [Opcode.ofNat, Nat.ble, Nat.beq]
-    have h32 : Main[32] = 1 := (sub_eq_zero.mp (alu.2.2.1.resolve_right (by decide))).symm
-    exact (alu.2.2.2.1 (by rw [h32]; decide)).2.1
+def sp1_op_a : BitVec 5 := BitVec.ofNat 5 Main[6]
 
-def sp1_op_b : BitVec 5 :=
-  by
-    have _ := Main
-    have _ := cstrs
-    have _ := h_is_sltu
-    stop
-    refine BitVec.ofNatLT Main[14] ?_
-    simp
-    change Main[14] < 32
-    rw [SP1ConstraintList.allHold, allHold_constraints_iff_sltu h_is_sltu] at cstrs
-    obtain ⟨ lt_op, cpu, alu, rest ⟩ := cstrs
-    simp [ALUTypeReader.constraints, SP1Constraint.toProp] at alu
-    simp_all [Opcode.ofNat, Nat.ble, Nat.beq]
-    have h32 : Main[32] = 1 := (sub_eq_zero.mp (alu.2.2.1.resolve_right (by decide))).symm
-    exact (alu.2.2.2.1 (by rw [h32]; decide)).1.1
+def sp1_op_b : BitVec 5 := BitVec.ofNat 5 Main[14]
 
-def sp1_op_c : BitVec 5 :=
-  by
-    have _ := Main
-    have _ := cstrs
-    have _ := h_is_sltu
-    stop
-    refine BitVec.ofNatLT Main[21] ?_
-    simp
-    change Main[21] < 32
-    rw [SP1ConstraintList.allHold, allHold_constraints_iff_sltu h_is_sltu] at cstrs
-    obtain ⟨ lt_op, cpu, alu, rest ⟩ := cstrs
-    simp [ALUTypeReader.constraints, SP1Constraint.toProp] at alu
-    simp_all [Opcode.ofNat, Nat.ble, Nat.beq]
-    have h32 : Main[32] = 1 := (sub_eq_zero.mp (alu.2.2.1.resolve_right (by decide))).symm
-    exact (alu.2.2.2.1 (by rw [h32]; decide)).1.2.1
+def sp1_op_c : BitVec 12 := BitVec.ofNat 12 Main[21].val
 
 def sp1_slti : SailM Unit := do
-  let op_a := sp1_op_a Main cstrs h_is_sltu
+  let op_a := sp1_op_a Main
   Sail.writeReg Register.nextPC (Word.toBitVec64 #v[Main[3] + 4, Main[4], Main[5], 0])
   Sail.write_reg op_a (Word.toBitVec64 #v[Main[34], 0, 0, 0])
 
@@ -150,61 +103,39 @@ theorem correct_slti
   (cstrs : (constraints Main).allHold)
   (h_is_slti : is_slti Main)
   (state_cstrs : (constraints Main).initialState s) :
-  let op_c := sp1_op_c Main cstrs h_is_sltu
-  let op_b := sp1_op_b Main cstrs h_is_sltu
-  let op_a := sp1_op_a Main cstrs h_is_sltu
-  (spec_slti op_c (.Regidx op_b) (.Regidx op_a)).run s = (sp1_slti Main cstrs h_is_sltu).run s
+  let op_c := sp1_op_c Main
+  let op_b := sp1_op_b Main
+  let op_a := sp1_op_a Main
+  (spec_slti op_c (.Regidx op_b) (.Regidx op_a)).run s = (sp1_slti Main).run s
   := by
-    have _ := state_cstrs
-    have _ := cstrs
-    have _ := h_is_slti
-    stop
-    have h21 : Main[21].val < 32 := by
-      rw [SP1ConstraintList.allHold, allHold_constraints_iff_sltu h_is_sltu] at cstrs
-      obtain ⟨ lt_op, cpu, alu, rest ⟩ := cstrs
-      simp [ALUTypeReader.constraints, SP1Constraint.toProp] at alu
-      simp_all [Opcode.ofNat, Nat.ble, Nat.beq]
-    have h632 : Main[6].val < 32 := by
-      rw [SP1ConstraintList.allHold, allHold_constraints_iff_sltu h_is_sltu] at cstrs
-      obtain ⟨ lt_op, cpu, alu, rest ⟩ := cstrs
-      simp [ALUTypeReader.constraints, SP1Constraint.toProp] at alu
-      simp_all [Opcode.ofNat, Nat.ble, Nat.beq]
     simp [SP1ConstraintList.allHold] at cstrs; simp [is_slti] at h_is_slti
     rw [allHold_constraints_iff_slti h_is_slti] at cstrs
-    obtain ⟨lt_op_cstrs, cpu_cstrs, alu_cstrs, M33⟩ := cstrs
+    obtain ⟨lt_op_cstrs, cpu_cstrs, alu_cstrs, M33, _M13⟩ := cstrs
     have h_is_real : Main[32] + Main[33] = 1 := by simp_all
     rw [CPUState.allHold_constraints_iff_is_real h_is_real] at cpu_cstrs
     rw [ALUTypeReader.allHold_constraints_iff_is_real h_is_real] at alu_cstrs
-    obtain ⟨ _, trusted_instr_prop, _, _, ⟨ c0, c1, c2, c3 ⟩, _, _, _, _, _, _, _, _, _, _, _, is_U64_a, is_U64_b, is_U64_c , _, _ ⟩ := alu_cstrs
+    obtain ⟨ trusted_instr_prop, _, _, ⟨ c0, c1, c2, c3 ⟩, _, _, _, _, _, _, _, _, _, _, _, is_U64_a, is_U64_b, is_U64_c , _, _ ⟩ := alu_cstrs
     simp [SP1ConstraintList.initialState, constraints, SP1Constraint.toStateProp, List.Forall, CPUState.constraints, ALUTypeReader.constraints] at state_cstrs
     obtain ⟨throwaway, read_pc, read_op_a, read_op_b, read_op_c⟩ := state_cstrs
     clear throwaway; simp_all
-    simp [Opcode.ofNat, Nat.ble, Nat.beq] at *
+    simp [Opcode.ofNat, Nat.ble, Nat.beq] at *; simp_all [BitVec.ofNatLT_eq_ofNat]
     have is_U64_c : Word.isU64 #v[Main[21], Main[22], Main[23], Main[24]]
       := by apply Word.isU64_of_cases c0 c1 c2 c3
     obtain ⟨ h_f, h_imm_c ⟩ := trusted_instr_prop
-    have h_imm' : setWidth 12 (BitVec.ofNat 5 ↑Main[21]) = BitVec.ofNat 12 Main[21] := by
-      simp [setWidth, setWidth', BitVec.ofNatLT_eq_ofNat]
-      grind
-    simp [h_f] at read_op_b
     simp [spec_slti, sp1_slti, execute, execute_ITYPE']
     rw [Sail.run_readReg, read_pc]
     simp [sp1_op_a, sp1_op_b, sp1_op_c, read_op_b, read_op_a]
-    simp [BitVec.ofNatLT_eq_ofNat, h_imm', ← h_imm_c]
+    simp [← h_imm_c]
     rw [exec_ITYPE_pure_bv_to_w _ _ _ is_U64_b is_U64_c]
     simp [execute_ITYPE_pure_w]
-    by_cases h_is_op_a_0 : Main[6] = 0 <;> simp_all
-    · simp [Word.toBitVec64, Word.toNat]
-      exact Fin.BitVec_ofNat_add_eq_add_ofNat _ 4 (by decide) (by omega)
-    · have h6' : BitVec.ofNat 5 Main[6].val ≠ 0#5 := by
-        simp [← BitVec.toNat_inj]
-        clear *- h_is_op_a_0 h632
-        omega
-      simp [h6']
-      simp [Word.toBitVec64, Word.toNat]
-      apply LtOperationSigned.spec.signed is_U64_b is_U64_c at lt_op_cstrs
-      simp at lt_op_cstrs
-      simp [lt_op_cstrs]
+    by_cases h_is_op_a_0 : Main[6] = 0
+    · simp_all
+    · simp_all
+      rw [if_neg (by simp [← BitVec.toNat_inj]; omega)]
+      rw [if_neg (c := BitVec.ofNat 5 ↑Main[6] = 0#5) (by simp [← BitVec.toNat_inj]; omega)]
+      apply LtOperationSigned.spec.signed at lt_op_cstrs <;>
+      [ simp_all; exact is_U64_b; exact is_U64_c ]
+      simp_all [Word.toBitVec64, Word.toNat]
       rw [Fin.BitVec_ofNat_add_eq_add_ofNat _ 4 (by decide) (by omega)]
       simp [bitVecToRegidxVal]
 
@@ -217,63 +148,20 @@ open Lt
 variable
   (Main : Vector (Fin KB) 44)
   (s : SailState)
-  (cstrs : (constraints Main).allHold)
-  (h_is_sltu : is_sltu Main)
 
 def spec_sltu (rs2 rs1 rd : regidx) : SailM Unit := do
   Sail.writeReg Register.nextPC ((← Sail.readReg Register.PC) + 4#64)
   _ ← execute_RTYPE rs2 rs1 rd rop.SLTU
   pure ()
 
-def sp1_op_a : BitVec 5 :=
-  by
-    have _ := Main
-    have _ := cstrs
-    have _ := h_is_sltu
-    stop
-    refine BitVec.ofNatLT Main[6] ?_
-    change Main[6] < 32
-    rw [SP1ConstraintList.allHold, allHold_constraints_iff_sltu h_is_sltu] at cstrs
-    obtain ⟨ lt_op, cpu, alu, rest ⟩ := cstrs
-    simp [ALUTypeReader.constraints, SP1Constraint.toProp] at alu
-    simp_all [Opcode.ofNat, Nat.ble, Nat.beq]
-    have h32 : Main[32] = 1 := (sub_eq_zero.mp (alu.2.2.1.resolve_right (by decide))).symm
-    exact (alu.2.2.2.1 (by rw [h32]; decide)).2.1
+def sp1_op_a : BitVec 5 := BitVec.ofNat 5 Main[6]
 
-def sp1_op_b : BitVec 5 :=
-  by
-    have _ := Main
-    have _ := cstrs
-    have _ := h_is_sltu
-    stop
-    refine BitVec.ofNatLT Main[14] ?_
-    simp
-    change Main[14] < 32
-    rw [SP1ConstraintList.allHold, allHold_constraints_iff_sltu h_is_sltu] at cstrs
-    obtain ⟨ lt_op, cpu, alu, rest ⟩ := cstrs
-    simp [ALUTypeReader.constraints, SP1Constraint.toProp] at alu
-    simp_all [Opcode.ofNat, Nat.ble, Nat.beq]
-    have h32 : Main[32] = 1 := (sub_eq_zero.mp (alu.2.2.1.resolve_right (by decide))).symm
-    exact (alu.2.2.2.1 (by rw [h32]; decide)).1.1
+def sp1_op_b : BitVec 5 := BitVec.ofNat 5 Main[14]
 
-def sp1_op_c : BitVec 5 :=
-  by
-    have _ := Main
-    have _ := cstrs
-    have _ := h_is_sltu
-    stop
-    refine BitVec.ofNatLT Main[21] ?_
-    simp
-    change Main[21] < 32
-    rw [SP1ConstraintList.allHold, allHold_constraints_iff_sltu h_is_sltu] at cstrs
-    obtain ⟨ lt_op, cpu, alu, rest ⟩ := cstrs
-    simp [ALUTypeReader.constraints, SP1Constraint.toProp] at alu
-    simp_all [Opcode.ofNat, Nat.ble, Nat.beq]
-    have h32 : Main[32] = 1 := (sub_eq_zero.mp (alu.2.2.1.resolve_right (by decide))).symm
-    exact (alu.2.2.2.1 (by rw [h32]; decide)).1.2.1
+def sp1_op_c : BitVec 5 := BitVec.ofNat 5 Main[21]
 
 def sp1_sltu : SailM Unit := do
-  let op_a := sp1_op_a Main cstrs h_is_sltu
+  let op_a := sp1_op_a Main
   Sail.writeReg Register.nextPC (Word.toBitVec64 #v[Main[3] + 4, Main[4], Main[5], 0])
   Sail.write_reg op_a (Word.toBitVec64 #v[Main[34], 0, 0, 0])
 
@@ -281,37 +169,36 @@ set_option maxHeartbeats 1000000 in
 
 -- correctness proof across slt/slti/sltu/sltiu arms
 theorem correct_sltu
+  (cstrs : (constraints Main).allHold)
+  (h_is_sltu : is_sltu Main)
   (state_cstrs : (constraints Main).initialState s) :
-  let op_c := sp1_op_c Main cstrs h_is_sltu
-  let op_b := sp1_op_b Main cstrs h_is_sltu
-  let op_a := sp1_op_a Main cstrs h_is_sltu
-  (spec_sltu (.Regidx op_c) (.Regidx op_b) (.Regidx op_a)).run s = (sp1_sltu Main cstrs h_is_sltu).run s
+  let op_c := sp1_op_c Main
+  let op_b := sp1_op_b Main
+  let op_a := sp1_op_a Main
+  (spec_sltu (.Regidx op_c) (.Regidx op_b) (.Regidx op_a)).run s = (sp1_sltu Main).run s
   := by
-    have _ := state_cstrs
-    stop
     simp [SP1ConstraintList.allHold] at cstrs; simp [is_sltu] at h_is_sltu
     rw [allHold_constraints_iff_sltu h_is_sltu] at cstrs
-    obtain ⟨lt_op_cstrs, cpu_cstrs, alu_cstrs, M33⟩ := cstrs
+    obtain ⟨lt_op_cstrs, cpu_cstrs, alu_cstrs, M32, _M13⟩ := cstrs
     have h_is_real : Main[32] + Main[33] = 1 := by simp_all
     rw [CPUState.allHold_constraints_iff_is_real h_is_real] at cpu_cstrs
     rw [ALUTypeReader.allHold_constraints_iff_is_real h_is_real] at alu_cstrs
-    obtain ⟨ _, trusted_instr_prop, _, _, _, _, _, _, _, _, _, _, _, _, _, _, is_U64_a, is_U64_b, is_U64_c , _, _ ⟩ := alu_cstrs
+    obtain ⟨ trusted_instr_prop, _, _, _, _, _, _, _, _, _, _, _, _, _, _, is_U64_a, is_U64_b, is_U64_c , _, _ ⟩ := alu_cstrs
     simp [SP1ConstraintList.initialState, constraints, SP1Constraint.toStateProp, List.Forall, CPUState.constraints, ALUTypeReader.constraints] at state_cstrs
     obtain ⟨throwaway, read_pc, read_op_a, read_op_b, read_op_c⟩ := state_cstrs
     clear throwaway; simp_all
-    simp [Opcode.ofNat, Nat.ble, Nat.beq] at *; simp_all
+    simp [Opcode.ofNat, Nat.ble, Nat.beq] at *; simp_all [BitVec.ofNatLT_eq_ofNat]
     obtain ⟨ _, _, is_U64_c ⟩ := is_U64_c
     -- Now the monadic manipulation
     simp [spec_sltu, sp1_sltu, execute, execute_RTYPE']
     rw [Sail.run_readReg, read_pc]
     simp [sp1_op_a, sp1_op_b, sp1_op_c, read_op_b, read_op_c]
     rw [exec_RTYPE_pure_bv_to_w _ _ _ (by omega) (by omega)]
-    simp [execute_RTYPEW_pure_w]
-    by_cases h_is_op_a_0 : Main[6] = 0 <;> simp_all
-    · simp [Word.toBitVec64, Word.toNat]
-      exact Fin.BitVec_ofNat_add_eq_add_ofNat _ 4 (by decide) (by omega)
-    · rw [if_neg (by simpa [← BitVec.toNat_inj])]
-      rw [if_neg (c := (Main[6])#'_ = 0#5) (by simpa [← BitVec.toNat_inj])]
+    by_cases h_is_op_a_0 : Main[6] = 0
+    · simp_all
+    · simp_all
+      rw [if_neg (by simp [← BitVec.toNat_inj]; omega)]
+      rw [if_neg (c := BitVec.ofNat 5 ↑Main[6] = 0#5) (by simp [← BitVec.toNat_inj]; omega)]
       apply LtOperationSigned.spec.unsigned at lt_op_cstrs <;>
       [ simp_all; exact is_U64_b; exact is_U64_c ]
       simp_all [Word.toBitVec64, Word.toNat]
@@ -327,75 +214,46 @@ open Lt
 variable
   (Main : Vector (Fin KB) 44)
   (s : SailState)
-  (cstrs : (constraints Main).allHold)
-  (h_is_sltiu : is_sltiu Main)
 
 def spec_sltiu (imm : BitVec 12) (rs1 rd : regidx) : SailM Unit := do
   Sail.writeReg Register.nextPC ((← Sail.readReg Register.PC) + 4#64)
   _ ← execute_ITYPE imm rs1 rd iop.SLTIU
   pure ()
 
-def sp1_op_a : BitVec 5 :=
-  by
-    have _ := Main
-    have _ := cstrs
-    have _ := h_is_sltiu
-    stop
-    refine BitVec.ofNatLT Main[6] ?_
-    change Main[6] < 32
-    rw [SP1ConstraintList.allHold, allHold_constraints_iff_sltiu h_is_sltiu] at cstrs
-    obtain ⟨ lt_op, cpu, alu, rest ⟩ := cstrs
-    simp [ALUTypeReader.constraints, SP1Constraint.toProp] at alu
-    simp_all [Opcode.ofNat, Nat.ble, Nat.beq]
-    have h32 : Main[32] = 1 := (sub_eq_zero.mp (alu.2.2.1.resolve_right (by decide))).symm
-    exact (alu.2.2.2.1 (by rw [h32]; decide)).2.1
+def sp1_op_a : BitVec 5 := BitVec.ofNat 5 Main[6]
 
-def sp1_op_b : BitVec 5 :=
-  by
-    have _ := Main
-    have _ := cstrs
-    have _ := h_is_sltiu
-    stop
-    refine BitVec.ofNatLT Main[14] ?_
-    simp
-    change Main[14] < 32
-    rw [SP1ConstraintList.allHold, allHold_constraints_iff_sltiu h_is_sltiu] at cstrs
-    obtain ⟨ lt_op, cpu, alu, rest ⟩ := cstrs
-    simp [ALUTypeReader.constraints, SP1Constraint.toProp] at alu
-    simp_all [Opcode.ofNat, Nat.ble, Nat.beq]
-    have h32 : Main[32] = 1 := (sub_eq_zero.mp (alu.2.2.1.resolve_right (by decide))).symm
-    exact (alu.2.2.2.1 (by rw [h32]; decide)).1.1
+def sp1_op_b : BitVec 5 := BitVec.ofNat 5 Main[14]
 
 def sp1_op_c : BitVec 12 := BitVec.ofNat 12 Main[21].val
 
 def sp1_sltiu : SailM Unit := do
-  let op_a := sp1_op_a Main cstrs h_is_sltiu
+  let op_a := sp1_op_a Main
   Sail.writeReg Register.nextPC (Word.toBitVec64 #v[Main[3] + 4, Main[4], Main[5], 0])
   Sail.write_reg op_a (Word.toBitVec64 #v[Main[34], 0, 0, 0])
 
 set_option maxHeartbeats 1000000 in
 
 -- correctness proof across slt/slti/sltu/sltiu arms
-theorem correct_sltu
+theorem correct_sltiu
+  (cstrs : (constraints Main).allHold)
+  (h_is_sltiu : is_sltiu Main)
   (state_cstrs : (constraints Main).initialState s) :
   let op_c := sp1_op_c Main
-  let op_b := sp1_op_b Main cstrs h_is_sltiu
-  let op_a := sp1_op_a Main cstrs h_is_sltiu
-  (spec_sltiu op_c (.Regidx op_b) (.Regidx op_a)).run s = (sp1_sltiu Main cstrs h_is_sltiu).run s
+  let op_b := sp1_op_b Main
+  let op_a := sp1_op_a Main
+  (spec_sltiu op_c (.Regidx op_b) (.Regidx op_a)).run s = (sp1_sltiu Main).run s
   := by
-    have _ := state_cstrs
-    stop
     simp [SP1ConstraintList.allHold] at cstrs; simp [is_sltiu] at h_is_sltiu
     rw [allHold_constraints_iff_sltiu h_is_sltiu] at cstrs
-    obtain ⟨lt_op_cstrs, cpu_cstrs, alu_cstrs, M33⟩ := cstrs
+    obtain ⟨lt_op_cstrs, cpu_cstrs, alu_cstrs, M32, _M13⟩ := cstrs
     have h_is_real : Main[32] + Main[33] = 1 := by simp_all
     rw [CPUState.allHold_constraints_iff_is_real h_is_real] at cpu_cstrs
     rw [ALUTypeReader.allHold_constraints_iff_is_real h_is_real] at alu_cstrs
-    obtain ⟨ _, trusted_instr_prop, _, _, ⟨ c0, c1, c2, c3 ⟩, _, _, _, _, _, _, _, _, _, _, _, is_U64_a, is_U64_b, is_U64_c , _, _ ⟩ := alu_cstrs
+    obtain ⟨ trusted_instr_prop, _, _, ⟨ c0, c1, c2, c3 ⟩, _, _, _, _, _, _, _, _, _, _, _, is_U64_a, is_U64_b, is_U64_c , _, _ ⟩ := alu_cstrs
     simp [SP1ConstraintList.initialState, constraints, SP1Constraint.toStateProp, List.Forall, CPUState.constraints, ALUTypeReader.constraints] at state_cstrs
     obtain ⟨throwaway, read_pc, read_op_a, read_op_b, read_op_c⟩ := state_cstrs
     clear throwaway; simp_all
-    simp [Opcode.ofNat, Nat.ble, Nat.beq] at *; simp_all
+    simp [Opcode.ofNat, Nat.ble, Nat.beq] at *; simp_all [BitVec.ofNatLT_eq_ofNat]
     have is_U64_c : Word.isU64 #v[Main[21], Main[22], Main[23], Main[24]]
       := by apply Word.isU64_of_cases c0 c1 c2 c3
     obtain ⟨ h_f, h_imm_c ⟩ := trusted_instr_prop
@@ -406,11 +264,11 @@ theorem correct_sltu
     rw [← h_imm_c]
     rw [exec_ITYPE_pure_bv_to_w _ _ _ is_U64_b is_U64_c]
     simp [execute_ITYPE_pure_w]
-    by_cases h_is_op_a_0 : Main[6] = 0 <;> simp_all
-    · simp [Word.toBitVec64, Word.toNat]
-      exact Fin.BitVec_ofNat_add_eq_add_ofNat _ 4 (by decide) (by omega)
-    · rw [if_neg (by simpa [← BitVec.toNat_inj])]
-      rw [if_neg (c := (Main[6])#'_ = 0#5) (by simpa [← BitVec.toNat_inj])]
+    by_cases h_is_op_a_0 : Main[6] = 0
+    · simp_all
+    · simp_all
+      rw [if_neg (by simp [← BitVec.toNat_inj]; omega)]
+      rw [if_neg (c := BitVec.ofNat 5 ↑Main[6] = 0#5) (by simp [← BitVec.toNat_inj]; omega)]
       apply LtOperationSigned.spec.unsigned at lt_op_cstrs <;>
       [ simp_all; exact is_U64_b; exact is_U64_c ]
       simp_all [Word.toBitVec64, Word.toNat]
