SP1Chips/Mul/Constraints.lean
@@ -99,7 +99,7 @@ lemma allHold_constraints_iff :
   List.Forall SP1Constraint.toProp (constraints Main) ↔
     List.Forall SP1Constraint.toProp (MulOperation.constraints #v[Main[28], Main[29], Main[30], Main[31]] #v[Main[15], Main[16], Main[17], Main[18]] #v[Main[22], Main[23], Main[24], Main[25]] { carry := #v[Main[32], Main[33], Main[34], Main[35], Main[36], Main[37], Main[38], Main[39], Main[40], Main[41], Main[42], Main[43], Main[44], Main[45], Main[46], Main[47]], product := #v[Main[48], Main[49], Main[50], Main[51], Main[52], Main[53], Main[54], Main[55], Main[56], Main[57], Main[58], Main[59], Main[60], Main[61], Main[62], Main[63]], b_lower_byte := { low_bytes := #v[Main[64], Main[65], Main[66], Main[67]] }, c_lower_byte := { low_bytes := #v[Main[68], Main[69], Main[70], Main[71]] }, b_msb := Main[72], c_msb := Main[73], product_msb := { msb := Main[74] }, b_sign_extend := Main[75], c_sign_extend := Main[76] } (Main[77] + Main[78] + Main[79] + Main[80] + Main[81]) Main[77] Main[78] Main[81] Main[79] Main[80]) ∧
     List.Forall SP1Constraint.toProp (CPUState.constraints { clk_high := Main[0], clk_16_24 := Main[1], clk_0_16 := Main[2], pc := #v[Main[3], Main[4], Main[5]] } #v[Main[3] + 4, Main[4], Main[5]] 8 (Main[77] + Main[78] + Main[79] + Main[80] + Main[81])) ∧
-    List.Forall SP1Constraint.toProp (RTypeReader.constraints Main[0] (Main[2] + Main[1] * 65536) #v[Main[3], Main[4], Main[5]] (Main[77] * 11 + Main[78] * 12 + Main[79] * 13 + Main[80] * 14 + Main[81] * 47) #v[Main[77] * 8 + Main[78] * 8 + Main[79] * 8 + Main[80] * 8 + Main[81] * 8,
+    List.Forall SP1Constraint.toProp (RTypeReader.constraints Main[0] (Main[2] + Main[1] * 65536) #v[Main[3], Main[4], Main[5]] (Main[77] * 11 + Main[78] * 12 + Main[79] * 13 + Main[80] * 14 + Main[81] * 24) #v[Main[77] * 8 + Main[78] * 8 + Main[79] * 8 + Main[80] * 8 + Main[81] * 8,
           Main[77] * 51 + Main[78] * 51 + Main[79] * 51 + Main[80] * 51 + Main[81] * 59,
           Main[78] + Main[79] * 3 + Main[80] * 2, Main[77] + Main[78] + Main[79] + Main[80] + Main[81]] #v[Main[28], Main[29], Main[30], Main[31]] { op_a := Main[6], op_a_memory := { prev_value := #v[Main[7], Main[8], Main[9], Main[10]], access_timestamp := { prev_low := Main[11], diff_low_limb := Main[12] } }, op_a_0 := Main[13], op_b := Main[14], op_b_memory := { prev_value := #v[Main[15], Main[16], Main[17], Main[18]], access_timestamp := { prev_low := Main[19], diff_low_limb := Main[20] } }, op_c := Main[21], op_c_memory := { prev_value := #v[Main[22], Main[23], Main[24], Main[25]], access_timestamp := { prev_low := Main[26], diff_low_limb := Main[27] } }  } (Main[77] + Main[78] + Main[79] + Main[80] + Main[81])) ∧
     (Main[77] = 0 ∨ Main[77] = 1) ∧
@@ -107,9 +107,9 @@ lemma allHold_constraints_iff :
     (Main[79] = 0 ∨ Main[79] = 1) ∧
     (Main[81] = 0 ∨ Main[81] = 1) ∧
     (Main[80] = 0 ∨ Main[80] = 1) ∧
-    (Main[77] + Main[78] + Main[79] + Main[80] + Main[81] = 0 ∨ Main[77] + Main[78] + Main[79] + Main[80] + Main[81] - 1 = 0) --∧
+    (Main[77] + Main[78] + Main[79] + Main[80] + Main[81] = 0 ∨ Main[77] + Main[78] + Main[79] + Main[80] + Main[81] - 1 = 0) ∧
+    Main[13] = 0
   := by
-    stop
     simp [constraints, sub_eq_zero]
 
 section opcodes
@@ -127,7 +127,6 @@ lemma single_op : List.Forall SP1Constraint.toProp (constraints Main) →
   (Main[80] = 1 → Main[77] = 0 ∧ Main[78] = 0 ∧ Main[79] = 0 ∧ Main[81] = 0) ∧
   (Main[81] = 1 → Main[77] = 0 ∧ Main[78] = 0 ∧ Main[79] = 0 ∧ Main[80] = 0)
    := by
-  stop
   intro cstrs
   simp [allHold_constraints_iff] at cstrs
   obtain ⟨ h_mop, cpu, alu, b_mul, b_mulh, b_mulhu, b_mulhsu, b_mulw, rest ⟩ := cstrs
@@ -151,7 +150,6 @@ section entailed_constraints
 lemma register_bounds : List.Forall SP1Constraint.toProp (constraints Main) → is_real Main →
   Main[6] < 32 ∧ Main[14] < 32 ∧ (Main[30] = 0 → Main[21] < 32) ∧ Main[3] < 65536
     := by
-  stop
   intro cstrs real
   have ⟨ sop1, sop2, sop3, sop4, sop5 ⟩ := single_op Main cstrs
   simp [is_real] at real
@@ -160,13 +158,12 @@ lemma register_bounds : List.Forall SP1Constraint.toProp (constraints Main) → 
   clear h_mop cpu rest
   rw [RTypeReader.allHold_constraints_iff_is_real] at alu
   simp only at alu
-  · obtain ⟨ h0, h1, h2, h3, h4, h5, b_imm, h7, h8, h9 ⟩ := alu
-    rcases real with mul | mulh | mulhu | mulhsu | mulw <;> simp_all [Opcode.ofNat, Nat.ble, Nat.beq]
+  · obtain ⟨ h1, h2, h3, h4, h5, b_imm, h7, h8, h9 ⟩ := alu
+    rcases real with mul | mulh | mulhu | mulhsu | mulw <;> simp_all [Opcode.ofNat, Nat.ble]
   · clear alu; rcases real with mul | mulh | mulhu | mulhsu | mulw <;> simp_all
 
 lemma op_a_is_0 : List.Forall SP1Constraint.toProp (constraints Main) → is_real Main →
   (Main[6] = 0 → Main[28] = 0 ∧ Main[29] = 0 ∧ Main[30] = 0 ∧ Main[31] = 0) := by
-  stop
   intro cstrs real
   have ⟨ sop1, sop2, sop3, sop4, sop5 ⟩ := single_op Main cstrs
   simp [is_real] at real
@@ -175,14 +172,13 @@ lemma op_a_is_0 : List.Forall SP1Constraint.toProp (constraints Main) → is_rea
   clear h_mop cpu rest
   rw [RTypeReader.allHold_constraints_iff_is_real] at alu
   simp only at alu
-  · obtain ⟨ h0, h1, h2, h3, h4, h5, b_imm, h7, h8, h9 ⟩ := alu
+  · obtain ⟨ h1, h2, h3, h4, h5, b_imm, h7, h8, h9 ⟩ := alu
     intro hm6; simp_all
   · clear alu; rcases real with mul | mulh | mulhu | mulhsu | mulw <;> simp_all
 
 lemma ops_U64_b_c : List.Forall SP1Constraint.toProp (constraints Main) → is_real Main →
   Word.isU64 #v[Main[15], Main[16], Main[17], Main[18]] ∧
   Word.isU64 #v[Main[22], Main[23], Main[24], Main[25]] := by
-  stop
   intro cstrs real
   have ⟨ sop1, sop2, sop3, sop4, sop5 ⟩ := single_op Main cstrs
   simp [is_real] at real
@@ -190,7 +186,7 @@ lemma ops_U64_b_c : List.Forall SP1Constraint.toProp (constraints Main) → is_r
   obtain ⟨ h_mop, cpu, alu, b_mul, b_mulh, b_mulhu, b_mulhsu, b_mulw, rest ⟩ := cstrs
   clear h_mop cpu rest
   rw [RTypeReader.allHold_constraints_iff_is_real] at alu
-  · obtain ⟨ h0, h1, h2, h3, h4, h5, b_imm, h7, h8, h9 ⟩ := alu
+  · obtain ⟨ h1, h2, h3, h4, h5, b_imm, h7, h8, h9 ⟩ := alu
     simp_all
   · clear alu; rcases real with mul | mulh | mulhu | mulhsu | mulw <;> simp_all
 
@@ -200,7 +196,6 @@ section operands
 
 @[simp]
 def sp1_op_a : List.Forall SP1Constraint.toProp (constraints Main) → is_real Main → BitVec 5 := by
-  stop
   intro cstrs real
   refine BitVec.ofNatLT Main[6] ?_
   change Main[6] < 32
@@ -209,7 +204,6 @@ def sp1_op_a : List.Forall SP1Constraint.toProp (constraints Main) → is_real M
 
 @[simp]
 def sp1_op_b : List.Forall SP1Constraint.toProp (constraints Main) → is_real Main → BitVec 5 := by
-  stop
   intro cstrs real
   refine BitVec.ofNatLT Main[14] ?_
   change Main[14] < 32
@@ -218,7 +212,6 @@ def sp1_op_b : List.Forall SP1Constraint.toProp (constraints Main) → is_real M
 
 @[simp]
 def sp1_op_c : List.Forall SP1Constraint.toProp (constraints Main) → is_real Main → Main[30] = 0 → BitVec 5 := by
-  stop
   intro cstrs real imm
   refine BitVec.ofNatLT Main[21] ?_
   change Main[21] < 32
@@ -233,8 +226,6 @@ lemma spec.mul (h : is_mul Main) :
   List.Forall SP1Constraint.toProp (constraints Main) →
     Word.toBitVec64 #v[Main[28], Main[29], Main[30], Main[31]] = execute_MUL_pure_bw (Word.toBWord #v[Main[15], Main[16], Main[17], Main[18]]) (Word.toBWord #v[Main[22], Main[23], Main[24], Main[25]]) .MUL
   := by
-    have _ := h
-    stop
     intro cstrs
     obtain ⟨ eq_mul, eq_imm ⟩ := h
     have ⟨ is_U64_b, is_U64_c ⟩ := ops_U64_b_c Main cstrs (mul_real Main eq_mul)
@@ -253,8 +244,6 @@ lemma spec.mulh (h : is_mulh Main) :
   List.Forall SP1Constraint.toProp (constraints Main) →
     Word.toBitVec64 #v[Main[28], Main[29], Main[30], Main[31]] = execute_MUL_pure_bw (Word.toBWord #v[Main[15], Main[16], Main[17], Main[18]]) (Word.toBWord #v[Main[22], Main[23], Main[24], Main[25]]) .MULH
   := by
-    have _ := h
-    stop
     intro cstrs
     obtain ⟨ eq_mulh, eq_imm ⟩ := h
     have ⟨ is_U64_b, is_U64_c ⟩ := ops_U64_b_c Main cstrs (mulh_real Main eq_mulh)
@@ -273,8 +262,6 @@ lemma spec.mulhu (h : is_mulhu Main) :
   List.Forall SP1Constraint.toProp (constraints Main) →
     Word.toBitVec64 #v[Main[28], Main[29], Main[30], Main[31]] = execute_MUL_pure_bw (Word.toBWord #v[Main[15], Main[16], Main[17], Main[18]]) (Word.toBWord #v[Main[22], Main[23], Main[24], Main[25]]) .MULHU
   := by
-    have _ := h
-    stop
     intro cstrs
     obtain ⟨ eq_mulhu, eq_imm ⟩ := h
     have ⟨ is_U64_b, is_U64_c ⟩ := ops_U64_b_c Main cstrs (mulhu_real Main eq_mulhu)
@@ -293,8 +280,6 @@ lemma spec.mulhsu (h : is_mulhsu Main) :
   List.Forall SP1Constraint.toProp (constraints Main) →
     Word.toBitVec64 #v[Main[28], Main[29], Main[30], Main[31]] = execute_MUL_pure_bw (Word.toBWord #v[Main[15], Main[16], Main[17], Main[18]]) (Word.toBWord #v[Main[22], Main[23], Main[24], Main[25]]) .MULHSU
   := by
-    have _ := h
-    stop
     intro cstrs
     obtain ⟨ eq_mulhsu, eq_imm ⟩ := h
     have ⟨ is_U64_b, is_U64_c ⟩ := ops_U64_b_c Main cstrs (mulhsu_real Main eq_mulhsu)
@@ -313,8 +298,6 @@ lemma spec.mulw (h : is_mulw Main) :
   List.Forall SP1Constraint.toProp (constraints Main) →
     Word.toBitVec64 #v[Main[28], Main[29], Main[30], Main[31]] = execute_MULW_pure_bhw (Word.toBWord #v[Main[15], Main[16], Main[17], Main[18]]).low (Word.toBWord #v[Main[22], Main[23], Main[24], Main[25]]).low
   := by
-    have _ := h
-    stop
     intro cstrs
     obtain ⟨ eq_mulw, eq_imm ⟩ := h
     have ⟨ is_U64_b, is_U64_c ⟩ := ops_U64_b_c Main cstrs (mulw_real Main eq_mulw)
